Structures/OracleState.v
@@ -10,18 +10,52 @@ Set Implicit Arguments.
 From Probchain
 Require Import BlockChain InvMisc FixedList FixedMap.
 
-Parameter OracleState_size: nat.
+Parameter oraclestate_size: nat.
 
-Definition OracleState_keytype := [eqType of ([eqType of ([eqType of Hashed] * [eqType of BlockRecord])] * (ordinal Maximum_proof_of_work))%type].
-Definition OracleState := fixmap  OracleState_keytype  [eqType of Hashed] OracleState_size.
+Definition oraclestate_keytype := [eqType of ([eqType of ([eqType of Hashed] * [eqType of BlockRecord])] * (ordinal Maximum_proof_of_work))%type].
+Definition oraclestate := fixmap  oraclestate_keytype  [eqType of Hashed] oraclestate_size.
 
-Definition OracleState_new : OracleState := fixmap_empty OracleState_keytype [eqType of Hashed] OracleState_size.
-
-
-Definition OracleState_find k (m : OracleState) := fixmap_find k m.
+Definition oraclestate_new : oraclestate := fixmap_empty oraclestate_keytype [eqType of Hashed] oraclestate_size.
 
 
+Definition oraclestate_find k (m : oraclestate) := fixmap_find k m.
 
-Definition OracleState_put (k: OracleState_keytype) (v : Hashed) (m: OracleState) :=
+
+
+Definition oraclestate_put (k: oraclestate_keytype) (v : Hashed) (m: oraclestate) :=
   fixmap_put k v m.
+
+  About finmap_cancel.
+
+  Definition oraclestate_prod (m : oraclestate) := finmap_prod m.
+  Definition prod_oraclestate pair : oraclestate := prod_finmap pair.
+
+  Lemma oraclestate_cancel : cancel oraclestate_prod prod_oraclestate.
+  Proof.
+    by case.
+  Qed.
+
+
+  Definition oraclestate_eqMixin  :=
+  CanEqMixin oraclestate_cancel.
+  Canonical oraclestate_eqType :=
+  Eval hnf in EqType oraclestate oraclestate_eqMixin.
+
+
+  Definition oraclestate_choiceMixin  :=
+  CanChoiceMixin oraclestate_cancel.
+  Canonical oraclestate_choiceType :=
+  Eval hnf in ChoiceType oraclestate oraclestate_choiceMixin.
+
+  Definition oraclestate_countMixin :=
+  CanCountMixin oraclestate_cancel.
+  Canonical oraclestate_countType :=
+  Eval hnf in CountType oraclestate oraclestate_countMixin.
+  
+  Definition oraclestate_finMixin :=
+  CanFinMixin oraclestate_cancel.
+  Canonical oraclestate_finType :=
+  Eval hnf in FinType oraclestate oraclestate_finMixin.
+
+
 
